cryptis/core/term.v
@@ -1,2 +1,2 @@
 From cryptis.core Require Export pre_term.
-From cryptis.core.term Require Export base algebra repr nonces subterms spec.
+From cryptis.core.term Require Export base algebra tsize repr nonces subterms spec.
